\guard

\input{common/defns/sumOfSequence.tex}
\input{common/defns/productOfSequence.tex}

\begin{thm}
\label{thm:sumProductDistribution}
  Let $a$ and $b$ sequences with $\set{n,\dots,m}\subset\NN$ for some $n<m$ in $\NN$ and $c\in\RR$.
  Then,
  \begin{enumerate}
    \item $\left( \sum_{i=n}^m a_i\right) + \left( \sum_{i=n}^m b_i\right) = \sum_{i=n}^m (a_i + b_i)$,
    \item $c\sum_{i=n}^m a_i = \sum_{i=n}^m ca_i$, and
    \item $\left( \Pi_{i=n}^m a_i\right)\left( \Pi_{i=n}^m b_i\right) = \Pi_{i=n}^m a_ib_i$
  \end{enumerate}
\end{thm}
\begin{proof}
  %TODO: prove this
\end{proof}
