\guard

\input{setTheory/examples/easyInjectiveExamples.tex}
\input{setTheory/examples/easySurjectiveExamples.tex}

\input{setTheory/defns/bijection.tex}

\begin{exmp}
\label{exmp:easyBijectionExamples}
  \begin{enumerate}
    \item Show that $f(x) = 4x-1$ is a bijection.\\

    In Examples \ref{exmp:easyInjectiveExamples} and \ref{exmp:easySurjectiveExamples} respectively, we showed that $f$ is injective and surjective.
    So, as $f$ is both an injection and a surjection, $f$ is a bijection.

    \item Show that $g:\RR^2\to\RR^2$ defined by \[ g(x,y) = (x+y,x-y)\] is a bijection.\\

    First, we show that $g$ is injective.
    Fix $x,y,a,b\in\RR$ such that $g(x,y) = g(a,b)$.
    Then by definiton of $g$, we have that
    \begin{alignat*}{2}
      && g(x,y)&=g(a,b) \\
      &\Rightarrow\quad& (x+y,x-y) &= (a+b,a-b) \\
      &\Rightarrow\quad& (x+y = a+b)\wedge (x-y=a-b)\,.
    \end{alignat*}
    Adding these two equalities gives that $ 2x = 2a$.
    So, $x=a$.
    Now, as $x=a$ and $x+y = a+b$, we have that $y=b$.
    Thus, $(x,y)=(a,b)$.
    So $g$ is injective.

    Now, to show that $g$ is surjective.
    Fix $u,v\in\RR$.
    Let $x = \frac{u+v}{2}$ and $y=\frac{u-v}{2}$.
    Then, we can note that
    \begin{align*}
      g(x,y)  &= \left( \frac{u+v}{2}+\frac{u-v}{2}, \frac{u+v}{2}-\frac{u-v}{2} \right)\\
              &= \left( \frac{u+v+u-v}{2}, \frac{u+v-u+v}{2} \right)\\
              &= \left( \frac{2u}{2}, \frac{2v}{2} \right)\\
              &= \left( u, v \right)
    \end{align*}
    So, $g$ is injective.
  \end{enumerate}

\end{exmp}
