\guard

\input{common/defns/sumOfSequence.tex}

\begin{prop}
\label{prop:sumOfConsequtiveIntegers}
  \[\forall n\in\NN\quad\sum_{i=0}^n i = \frac{n(n+1)}{2}\,.\]
\end{prop}
\begin{proof}
  We'll prove this by induction on integers $n\in\NN$.

  Base step.
  By Definition \ref{defn:sumOfSequence} and some simple arithmatic, we have that
    \begin{align*}
      \sum_{i=0}^0 i  &= 0 \\
                      &= \frac{ 0(0+1)}{2}\,,
    \end{align*}
  and so the claim holds at $n=0$.

  Inductive step. Let $n\in\NN$ and suppose that $\sum_{i=0}^n i = \frac{n(n+1)}{2}$.
  Then, by Definition \ref{defn:sumOfSequence},
    \[ \sum_{i=0}^{n+1} i = \left( \sum_{i=0}^{n} i \right) + (n+1)\,. \]
  Now, using our inductive hypothesis we have
    \begin{align*}
      \sum_{i=0}^{n+1} i &= \left( \sum_{i=0}^{n} i \right) + (n+1) \\
                         &= \frac{ n(n+1)}{2} + (n+1) \\
                         &= \frac{ n(n+1)}{2} + \frac{2(n+1)}{2} \\
                         &= \frac{ n(n+1)+2(n+1)}{2} \\
                         &= \frac{ (n+1)(n+2) }{2} \,.
    \end{align*}
\end{proof}
