\guard

\input{setTheory/props/functionEquality.tex}
\input{setTheory/defns/functionInverse.tex}
\input{setTheory/defns/functionComposition.tex}


\begin{prop}
\label{prop:inverseOfFunction}
  If $f:X\to Y$ is a bijection with inverse $f^{-1}:Y\to X$, then $f^{-1}\circ f=\id_X$.
\end{prop}
\begin{proof}
  Fix $f:X\to Y$ a bijection.
  Fix $x\in X$.
  Set $y=f(x)$.
  By definition of $f^{-1}$, $f^{-1}(y) = x$.
  So, we have that
  \begin{align*}
    (f^{-1}\circ f )(x) &= f^{-1}(f(x)) \\
                        &= f^{-1}(y) \\
                        &= x\,.
  \end{align*}
  Though, as $x\in X$ was arbitrary, we have that $\forall x\in X( f^{-1}\circ f=\id_X)$.
  Thus, by Proposition \ref{prop:functionEquality}, $f^{-1}\circ f=\id_X$.
\end{proof}
