\guard

\input{setTheory/defns/bijection.tex}
\input{setTheory/defns/inverse.tex}

\begin{prop}
\label{prop:inverseOfBijectionIsBijection}
  If $f:X\to Y$ is a bijections, then $f^{-1}$ is a bijection.
\end{prop}
\begin{proof}
  Fix $f:X\to Y$ a bijection.
  We must show that $f^{-1}$ is an injection and a surjection.

  To show that $f^{-1}:Y\to X$ is an injection, fix $y_1,y_2\in Y$.
  Suppose that $f^{-1}(y_1)=f^{-1}(y_2)$.
  Set $x = f^{-1}(y_1)\in X$.
  By definition of $f^{-1}$, $f(x)=y_1$
  Further, as $f^{-1}(y_1)=f^{-1}(y_2)$, $x = f^{-1}(y_2)$.
  Whence, $f(x)=y_2$.
  So, as $f(x)=y_1$ and $f(x)=y_2$, $y_1=y_2$.

  To show that $f^{-1}$ is a surjection, fix some $x\in X$.
  Now, set $y=f(x)$.
  Then, by definition of $f^{-1}$, $f^{-1}(y)=x$.
\end{proof}
