\guard

\input{common/defns/sequence.tex}

\begin{exmp}
\label{exmp:recurrenceRelation}
  Define the sequence $s$ as \[ s_0=0,~s_1=4,s_k=6s_{k-1}-5s_{k-2}\,.\]
  We want to show that $\forall n\in\NN$ $s_n = 5^n-1$.

  We do so by strong induction on $n\in\NN$.

  Base step, we check that the claim holds for $n=0$ and $n=1$.
  Here, we note that $s_0 = 0 = 5^0-1$ and $s_1 = 4 = 5^1-1$.
  So, the claim holds at the first two values for $n$.

  Now, we check the inductive step.
  Let $n\in\NN$ and suppose that for all $k\in\NN$ with $k\leq n$ $s_k = 5^k-1$.
  Now, by definition $s_{n+1} = 6 s_n - 5 s_{n-1}$.
  Though, out inductive hypothesis provides that $s_n = 5^n-1 $ and $s_{n-1}=5^{n-1}-1$.
  Thus,
  \begin{align*}
    s_{n+1} &= 6 s_n - 5 s_{n-1} \\
            &= 6 ( 5^n - 1 ) - 5 ( 5^{n-1} - 1 ) \\
            &= 6\cdot 5^n - 6 - 5^n - 5 \\
            &= 5\cdot 5^n - 1 \\
            &= 5^{n+1} - 1\,.
  \end{align*}
  showing that the claim holds at $n+1$.

  Thus, by induction, we have that $\forall n\in\NN$ $s_n = 5^n-1$.
\end{exmp}
