\guard

\input{logic/defns/negation.tex}
\input{logic/defns/disjunction.tex}
\input{logic/defns/conjunction.tex}
\input{logic/defns/conditional.tex}
\input{logic/defns/statementForm.tex}
\input{logic/defns/logicallyEquivalentStatementForm.tex}
\input{logic/props/doubleNegation.tex}
\input{logic/props/deMorgans.tex}

\begin{exmp}
\label{exmp:conditionalNegation}
  From Proposition \ref{prop:conditionEquivalence}, we have that $p\rightarrow q \equiv \neg p \vee q$.
  Applying DeMorgan's Law, Proposition \ref{prop:DeMorgans}, and using double negation, Proposition \ref{prop:doubleNegation}, we have that
  \begin{align}
    \neg (p \rightarrow q)  &\equiv \neg( \neg p \vee q ) \\
                            &\equiv \neg\neg p \wedge \neg q \\
                            &\equiv p \wedge \neg q\,.
  \end{align}
  Whence, $ \neg( p\rightarrow q ) \equiv p \wedge \neg q $.
\end{exmp}
